theories/simplang/gen_adequacy.v
@@ -1,36 +1,38 @@
 From simuliris.logic Require Import satisfiable.
 From simuliris.simulation Require Import slsls global_sim adequacy.
 From simuliris.simplang Require Import proofmode tactics behavior.
-From simuliris.simplang Require Import parallel_subst gen_val_rel.
+From simuliris.simplang Require Import parallel_subst gen_val_rel wf.
 
 (** Generic adequacy theorem for sheap-based logical relations. *)
 Section adequacy.
-  Lemma simplang_adequacy `{sheapGpreS Σ} p_t p_s g :
-    isat (∀ `(sheapGS Σ), |==> ∃ `(sheapInv Σ) loc_rel,
+  Lemma simplang_adequacy `{sheapGpreS Σ} p_t p_s:
+    isat (∀ `(sheapGS Σ) gs,
+      ⌜map_Forall (λ _ v, val_wf v) gs⌝ -∗
+      |==> ∃ `(sheapInv Σ) loc_rel,
       ([∗ map] f ↦ K ∈ p_t, f @t K) -∗
       ([∗ map] f ↦ K ∈ p_s, f @s K) -∗
-      ([∗ map] n↦v ∈ g, global_loc n ↦t v ∗ global_loc n …t 1 ∗ global_loc n ↦s v ∗ global_loc n …s 1) -∗
-      target_globals (dom _ g) -∗
-      source_globals (dom _ g) ==∗
-      sheap_inv p_s (state_init g) [Call f#"main" #()] ∗
+      ([∗ map] n↦v ∈ gs, global_loc n ↦t v ∗ global_loc n …t 1 ∗ global_loc n ↦s v ∗ global_loc n …s 1) -∗
+      target_globals (dom _ gs) -∗
+      source_globals (dom _ gs) ==∗
+      sheap_inv p_s (state_init gs) [Call f#"main" #()] ∗
       ext_rel 0 #() #() ∗
       (∀ v_t v_s, ext_rel 0 v_t v_s -∗ gen_val_rel loc_rel v_t v_s) ∗
       prog_rel p_t p_s
     ) →
-    beh_rel g p_t p_s.
+    beh_rel p_t p_s.
   Proof.
     intros Hrel. eapply (slsls_adequacy (sat:=isat)).
     eapply sat_mono, Hrel. clear Hrel.
-    iIntros "Hprog_rel %σ_t %σ_s".
+    iIntros "Hprog_rel %σ_t %σ_s (%gs&%&->&->)".
     iMod (sheap_init p_t _ p_s _) as (HsheapGS) "Hinit".
-    iMod ("Hprog_rel" $! HsheapGS) as (HsheapInv loc_rel) "Hprog_rel".
+    iMod ("Hprog_rel" $! HsheapGS gs with "[//]") as (HsheapInv loc_rel) "Hprog_rel".
     iDestruct ("Hinit" $! HsheapInv) as "(Hstate & Hp_t & Hmt_t & Hp_s & Hmt_s & Hg_s & Hg_t & Hprogs_are)".
     iMod ("Hprog_rel" with "Hp_t Hp_s [Hmt_t Hmt_s] Hg_t Hg_s") as "(Hinv & Hunit & Hobs & Hprog_rel)".
     { rewrite !big_sepM_sep. iFrame. }
     iModIntro. iExists sheapGS_simulirisGS.
     iFrame "Hprog_rel Hprogs_are Hunit".
     iSplitR "Hobs".
-    - iIntros ([-> ->]). iApply "Hstate". done.
+    - iApply "Hstate". done.
     - iIntros (??) "Hext". iApply gen_val_rel_obs. iApply "Hobs". done.
   Qed.
 
