theories/simplang/simple_inv/adequacy.v
@@ -23,25 +23,26 @@ Global Instance subG_sbijΣ Σ :
   subG simpleΣ Σ → simpleGpreS Σ.
 Proof. solve_inG. Qed.
 
-Lemma prog_rel_adequacy Σ `{!simpleGpreS Σ} (p_t p_s : prog) gs:
-  isat (∀ `(simpleGS Σ),
+Lemma prog_rel_adequacy Σ `{!simpleGpreS Σ} (p_t p_s : prog):
+  isat (∀ `(simpleGS Σ) gs,
+    ⌜map_Forall (λ _ v, val_wf v) gs⌝ -∗
     ([∗ map] f ↦ K ∈ p_t, f @t K) -∗
     ([∗ map] f ↦ K ∈ p_s, f @s K) -∗
     target_globals (dom (gset string) gs) -∗
     source_globals (dom (gset string) gs) ==∗
     ([∗ map] v∈gs, val_rel v v) ∗ prog_rel p_t p_s
   ) →
-  beh_rel gs p_t p_s.
+  beh_rel p_t p_s.
 Proof.
   intros Hprog. apply simplang_adequacy.
   eapply sat_mono, Hprog. clear Hprog.
-  iIntros "Hprog_rel %".
+  iIntros "Hprog_rel % %gs %".
   iMod (heapbij_init (λ _ _ q, q = Some 1%Qp)) as (?) "Hbij". iModIntro.
   set HΣ := (SimpleGS Σ _ _).
   iExists simple_inv, heapbij.loc_rel.
   iSpecialize ("Hprog_rel" $! HΣ).
   iIntros "Hp_t Hp_s Hmt #Hgs_t #Hgs_s".
-  iMod ("Hprog_rel" with "[$] [$] [$] [$]") as "[#Hvs $]".
+  iMod ("Hprog_rel" with "[//] [$] [$] [$] [$]") as "[#Hvs $]".
   iMod (heap_bij_insert_globals with "Hbij Hmt Hvs") as (L') "[Hbij #Hls]"; [done| ].
   iModIntro. iSplitL "Hbij"; [|iSplitR; [done|]].
   - iExists _, _. by iFrame "∗Hgs_t Hgs_s Hls".
@@ -53,9 +54,9 @@ Theorem log_rel_adequacy Σ `{!simpleGpreS Σ} e_t e_s :
   (∀ `(simpleGS Σ), ⊢ log_rel e_t e_s) →
   ctx_rel e_t e_s.
 Proof.
-  intros Hrel C fname x p gs Hpwf HCwf Hvars Hgs.
+  intros Hrel C fname x p Hpwf HCwf Hvars.
   apply (prog_rel_adequacy Σ). eapply isat_intro.
-  iIntros (?) "_ _ _ _ !#".
+  iIntros (? gs Hgs) "_ _ _ _ !#".
   iSplit. { iApply big_sepM_intro. iIntros "!>" (???). iApply val_wf_sound. by apply: Hgs. }
   iIntros "!# %f %K_s %π".
   iDestruct (Hrel _) as "Hrel". clear Hrel.
